Runtime/Utilities.lean
@@ -1,2 +1,3 @@
 import Runtime.Utilities.Extensions
+import Runtime.Utilities.Lean
 import Runtime.Utilities.SortedArray
