Runtime/Utilities/Lean.lean
@@ -1,0 +1,34 @@
+theorem Nat.zero_div_eq_zero : 0 / n = 0 := by
+  induction n
+  case zero => simp
+  case succ => rw [div_eq]; split <;> simp_all
+
+theorem Nat.mul_div_same_eq : (n : Nat) * m / m = n := by
+  induction n generalizing m
+  case zero => simp [zero_div_eq_zero]
+  case succ n hi => rw [Nat.mul_comm, mul_succ]; sorry
+
+instance [Ord α] : LE α := leOfOrd
+
+instance : DecidableEq Empty :=
+  fun empty _ => empty.casesOn
+
+@[reducible]
+instance [DecidableEq α] {β : α → Type _} [∀ a, DecidableEq (β a)] : DecidableEq (Σ a : α, β a) :=
+  fun ⟨a₁, b₁⟩ ⟨a₂, b₂⟩ => 
+    if h : a₁ = a₂ then 
+      if h' : (h ▸ b₁) = b₂ then
+        .isTrue (by subst h h'; rfl)
+      else 
+        .isFalse (by 
+          subst h
+          intro hc
+          injection hc
+          contradiction
+        )
+    else
+      .isFalse (by
+        intro hc
+        injection hc
+        contradiction
+      )
